clean sorted lemmas
- define sorted_cons'
- define sorted_rcons'

impredicative_set/.Makefile.coq.d
@@ -1,0 +1,36 @@
+imonae_lib.vo imonae_lib.glob imonae_lib.v.beautified imonae_lib.required_vo: imonae_lib.v 
+imonae_lib.vio: imonae_lib.v 
+imonae_lib.vos imonae_lib.vok imonae_lib.required_vos: imonae_lib.v 
+ihierarchy.vo ihierarchy.glob ihierarchy.v.beautified ihierarchy.required_vo: ihierarchy.v imonae_lib.vo
+ihierarchy.vio: ihierarchy.v imonae_lib.vio
+ihierarchy.vos ihierarchy.vok ihierarchy.required_vos: ihierarchy.v imonae_lib.vos
+imonad_lib.vo imonad_lib.glob imonad_lib.v.beautified imonad_lib.required_vo: imonad_lib.v imonae_lib.vo ihierarchy.vo
+imonad_lib.vio: imonad_lib.v imonae_lib.vio ihierarchy.vio
+imonad_lib.vos imonad_lib.vok imonad_lib.required_vos: imonad_lib.v imonae_lib.vos ihierarchy.vos
+ifail_lib.vo ifail_lib.glob ifail_lib.v.beautified ifail_lib.required_vo: ifail_lib.v imonae_lib.vo ihierarchy.vo imonad_lib.vo
+ifail_lib.vio: ifail_lib.v imonae_lib.vio ihierarchy.vio imonad_lib.vio
+ifail_lib.vos ifail_lib.vok ifail_lib.required_vos: ifail_lib.v imonae_lib.vos ihierarchy.vos imonad_lib.vos
+istate_lib.vo istate_lib.glob istate_lib.v.beautified istate_lib.required_vo: istate_lib.v imonae_lib.vo ihierarchy.vo imonad_lib.vo ifail_lib.vo
+istate_lib.vio: istate_lib.v imonae_lib.vio ihierarchy.vio imonad_lib.vio ifail_lib.vio
+istate_lib.vos istate_lib.vok istate_lib.required_vos: istate_lib.v imonae_lib.vos ihierarchy.vos imonad_lib.vos ifail_lib.vos
+itrace_lib.vo itrace_lib.glob itrace_lib.v.beautified itrace_lib.required_vo: itrace_lib.v ihierarchy.vo imonad_lib.vo
+itrace_lib.vio: itrace_lib.v ihierarchy.vio imonad_lib.vio
+itrace_lib.vos itrace_lib.vok itrace_lib.required_vos: itrace_lib.v ihierarchy.vos imonad_lib.vos
+imonad_composition.vo imonad_composition.glob imonad_composition.v.beautified imonad_composition.required_vo: imonad_composition.v imonae_lib.vo ihierarchy.vo imonad_lib.vo
+imonad_composition.vio: imonad_composition.v imonae_lib.vio ihierarchy.vio imonad_lib.vio
+imonad_composition.vos imonad_composition.vok imonad_composition.required_vos: imonad_composition.v imonae_lib.vos ihierarchy.vos imonad_lib.vos
+imonad_model.vo imonad_model.glob imonad_model.v.beautified imonad_model.required_vo: imonad_model.v imonae_lib.vo ihierarchy.vo imonad_lib.vo ifail_lib.vo istate_lib.vo itrace_lib.vo imonad_transformer.vo
+imonad_model.vio: imonad_model.v imonae_lib.vio ihierarchy.vio imonad_lib.vio ifail_lib.vio istate_lib.vio itrace_lib.vio imonad_transformer.vio
+imonad_model.vos imonad_model.vok imonad_model.required_vos: imonad_model.v imonae_lib.vos ihierarchy.vos imonad_lib.vos ifail_lib.vos istate_lib.vos itrace_lib.vos imonad_transformer.vos
+imonad_transformer.vo imonad_transformer.glob imonad_transformer.v.beautified imonad_transformer.required_vo: imonad_transformer.v imonae_lib.vo ihierarchy.vo imonad_lib.vo ifail_lib.vo istate_lib.vo
+imonad_transformer.vio: imonad_transformer.v imonae_lib.vio ihierarchy.vio imonad_lib.vio ifail_lib.vio istate_lib.vio
+imonad_transformer.vos imonad_transformer.vok imonad_transformer.required_vos: imonad_transformer.v imonae_lib.vos ihierarchy.vos imonad_lib.vos ifail_lib.vos istate_lib.vos
+ifmt_lifting.vo ifmt_lifting.glob ifmt_lifting.v.beautified ifmt_lifting.required_vo: ifmt_lifting.v imonae_lib.vo ihierarchy.vo imonad_lib.vo imonad_transformer.vo imonad_model.vo
+ifmt_lifting.vio: ifmt_lifting.v imonae_lib.vio ihierarchy.vio imonad_lib.vio imonad_transformer.vio imonad_model.vio
+ifmt_lifting.vos ifmt_lifting.vok ifmt_lifting.required_vos: ifmt_lifting.v imonae_lib.vos ihierarchy.vos imonad_lib.vos imonad_transformer.vos imonad_model.vos
+iparametricity_codensity.vo iparametricity_codensity.glob iparametricity_codensity.v.beautified iparametricity_codensity.required_vo: iparametricity_codensity.v imonae_lib.vo ihierarchy.vo imonad_lib.vo ifmt_lifting.vo imonad_model.vo
+iparametricity_codensity.vio: iparametricity_codensity.v imonae_lib.vio ihierarchy.vio imonad_lib.vio ifmt_lifting.vio imonad_model.vio
+iparametricity_codensity.vos iparametricity_codensity.vok iparametricity_codensity.required_vos: iparametricity_codensity.v imonae_lib.vos ihierarchy.vos imonad_lib.vos ifmt_lifting.vos imonad_model.vos
+iexample_transformer.vo iexample_transformer.glob iexample_transformer.v.beautified iexample_transformer.required_vo: iexample_transformer.v imonae_lib.vo ihierarchy.vo imonad_lib.vo ifail_lib.vo istate_lib.vo imonad_transformer.vo imonad_model.vo
+iexample_transformer.vio: iexample_transformer.v imonae_lib.vio ihierarchy.vio imonad_lib.vio ifail_lib.vio istate_lib.vio imonad_transformer.vio imonad_model.vio
+iexample_transformer.vos iexample_transformer.vok iexample_transformer.required_vos: iexample_transformer.v imonae_lib.vos ihierarchy.vos imonad_lib.vos ifail_lib.vos istate_lib.vos imonad_transformer.vos imonad_model.vos
